q

ZK_KE.ec
@@ -5,27 +5,24 @@ require import Ring StdRing StdOrder StdBigop Discrete RealSeq RealSeries RealLu
 (*---*) import IntOrder RealOrder RField.
 require (*--*) FinType.
 
+require import AllpairsProp.
 
 
-type ct,pt,rt, irt.
+type ct, pt, rt, irt.
 
 op d : ct distr.
 axiom duni : is_uniform d.
 
-search is_uniform.
-
-op umc : real.
-axiom ss c : mu1 d c = umc.
-
 op allcs : ct list.
 axiom allcs_uniq : uniq allcs.
 
+axiom ss c : mu1 d c = 1%r/(size allcs)%r.
 
 require BigPr.
-clone import BigPr as BP with type ct <- ct,
-                              type pt <- pt,
-                              type rt <- rt * rt,
-                              op d <- d,
+clone import BigPr as BP with type ct  <- ct,
+                              type pt  <- pt,
+                              type rt  <- rt * rt,
+                              op    d  <- d,
                               op allcs <- allcs.
 
 module type Adv = {
@@ -34,48 +31,34 @@ module type Adv = {
 }.
 
 
-lemma kiki2 ['a] : forall (l : 'a list), 
-  unzip1 (map (fun (x : 'a) => (x, x)) l) = l.
-elim. smt. smt.
-qed.
 
-lemma kiki3 ['a] x :  forall (l : 'a list), uniq l => !(x \in l) =>
- filter (fun x => fst x = snd x)  (map ((fun (c1 c2 : 'a) => (c1, c2)) x) l)  = [].
-elim. smt.
-progress. 
-smt.
-qed.
+module InitRun2(A : Adv) = {
+  proc run(a : pt) = {
+    var i, c1, c2, r1, r2;
+    i <- A.init(a);
+    
+    c1 <$ d;
+    r1 <- A.run(i,c1);
 
+    c2 <$ d;
+    r2 <- A.run(i,c2);
 
-lemma kiki4 ['a] x :  forall (l : 'a list), uniq l => x \in l =>
- filter (fun x => fst x = snd x)  (map ((fun (c1 c2 : 'a) => (c1, c2)) x) l)  = (x, x) :: [].
-elim. smt.
-move => y H2 H3 H4 H5. 
-case (x = y).
-move => H6. rewrite H6. simplify.
- have f : !(x \in H2). smt.
-apply  (kiki3 y). smt. smt.
-move => q. rewrite q. simplify. apply H3. smt. smt.
-qed.
+    return ((c1,r1),(c2,r2));
+  }
+}.
 
 
-lemma kiki0 ['a] : forall (l1 l2 : 'a list), size l1 <= size l2 => uniq l1 => uniq l2 => (forall x, x \in l1 => x \in l2) =>
-  (filter (fun x => fst x = snd x) (allpairs (fun (c1 c2 : 'a) => (c1, c2)) l1 l2)) = map (fun x => (x , x)) l1 .
-proof. elim. smt.
-progress. rewrite /cartprod2.
-rewrite allpairs_consl. simplify.
-rewrite filter_cat. 
-rewrite  (kiki4 x). auto. smt. simplify.
-smt (filter_cat kiki4).
-qed.
+module InitRun1(A : Adv) = {
+  proc run(a : pt) = {
+    var i, c1, r1;
+    i <- A.init(a);
+    
+    c1 <$ d;
+    r1 <- A.run(i,c1);
 
-
-lemma kiki ['a] (l : 'a list) : uniq l =>
-  unzip1 (filter (fun x => fst x = snd x) (cartprod2 l)) = l.
-move => q.
-rewrite /cartprod2.  rewrite kiki0;auto.
-rewrite kiki2. auto. 
-qed.
+    return (c1,r1);
+  }
+}.
 
 
 section.
@@ -113,21 +96,22 @@ local module X1 = {
 }.
 
 
-
+(* averging  *)
 local lemma x0 &m M p : 
-  big predT (fun (c : ct) => mu1 d c * Pr[C1.rest(p, c) @ &m : M c res]) allcs =
-     Pr[X1.run(p) @ &m : M res.`1 res.`2].
+  big predT (fun (c : ct) => mu1 d c * Pr[C1.rest(p, c) @ &m : M (c, res)]) allcs =
+     Pr[X1.run(p) @ &m : M (res.`1, res.`2)].
 admitted.
 
 
+(* c1c2 <$ d * d ~ c1 <$ d ; c2 <$ d  *)
 local lemma x1 &m M p: 
    Pr[X(C2).run(p) @ &m : M res] = Pr[Xseq(C2).run(p) @ &m : M res].
 admitted.
-
    
+(* sum binding  *)
 local lemma x2 &m M p:
-  Pr[X1.run(p) @ &m : M res.`1 res.`2] ^ 2 <=
-  Pr[Xseq(C2).run(p) @ &m : M res.`1.`1 res.`2.`1 /\ M res.`1.`2 res.`2.`2].
+  Pr[X1.run(p) @ &m : M (res.`1, res.`2)] ^ 2 <=
+  Pr[Xseq(C2).run(p) @ &m : M (res.`1.`1, res.`2.`1) /\ M (res.`1.`2, res.`2.`2)].
 admitted.
    
 
@@ -145,8 +129,8 @@ qed.
 
 
 local lemma avr_lemma_7_app &m M p c: 
- Pr[ C2.rest(p,(c,c)) @ &m :  M c res.`1 /\ M c res.`2 ]
-  <= Pr[ C1.rest(p,c) @ &m :  M c res ].
+ Pr[ C2.rest(p,(c,c)) @ &m :  M (c, res.`1) /\ M (c, res.`2) ]
+  <= Pr[ C1.rest(p,c) @ &m :  M (c, res) ].
 byequiv.
 proc.
 seq 2 2 : (={glob A,i,r1}).
@@ -157,26 +141,27 @@ qed.
 
 
 local lemma avr_lemma_8_app &m M p : 
-  Pr[ Xseq(C2).run(p) @ &m  : res.`1.`1 <> res.`1.`2 /\ M res.`1.`1 res.`2.`1 /\ M res.`1.`2 res.`2.`2 ] 
-     >= Pr[ Xseq(C2).run(p) @ &m  : M res.`1.`1 res.`2.`1 /\ M res.`1.`2 res.`2.`2  ] 
+  Pr[ Xseq(C2).run(p) @ &m  : res.`1.`1 <> res.`1.`2 /\ M (res.`1.`1, res.`2.`1) /\ M (res.`1.`2, res.`2.`2) ] 
+
+     >= Pr[ Xseq(C2).run(p) @ &m  : M (res.`1.`1, res.`2.`1) /\ M (res.`1.`2, res.`2.`2)  ] 
      - big (fun r => fst r = snd r)  (fun (c1c2 : ct * ct) => 
                   ((mu1 d c1c2.`1) * (mu1 d c1c2.`2)) * 
-                   Pr[ C1.rest(p,c1c2.`1) @ &m :  M c1c2.`1 res ]) 
+                   Pr[ C1.rest(p,c1c2.`1) @ &m :  M (c1c2.`1, res) ]) 
                    (cartprod2 allcs).
-rewrite (avr_lemma_6_app &m (fun (r :  (ct * ct) * (rt * rt)) =>   M r.`1.`1 r.`2.`1 /\ M r.`1.`2 r.`2.`2)).
+rewrite (avr_lemma_6_app &m (fun (r :  (ct * ct) * (rt * rt)) =>   M (r.`1.`1, r.`2.`1) /\ M (r.`1.`2, r.`2.`2))).
 simplify.
 have f2 :  big (fun (r : ct * ct) => r.`1 = r.`2)
   (fun (c1c2 : ct * ct) =>
      mu1 d c1c2.`1 * mu1 d c1c2.`2 *
-     Pr[C2.rest(p, c1c2) @ &m : M c1c2.`1 res.`1 /\ M c1c2.`2 res.`2])
+     Pr[C2.rest(p, c1c2) @ &m : M (c1c2.`1, res.`1) /\ M (c1c2.`2, res.`2)])
   (cartprod2 allcs) <= 
   big (fun (r : ct * ct) => r.`1 = r.`2)
   (fun (c1c2 : ct * ct) =>
      mu1 d c1c2.`1 * mu1 d c1c2.`2 *
-     Pr[C1.rest(p, c1c2.`1) @ &m : M c1c2.`1 res]) (cartprod2 allcs).
+     Pr[C1.rest(p, c1c2.`1) @ &m : M (c1c2.`1, res)]) (cartprod2 allcs).
 apply ler_sum. progress. 
-   have : Pr[C2.rest(p, a) @ &m : M a.`1 res.`1 /\ M a.`2 res.`2] <=
-            Pr[C1.rest(p, a.`1) @ &m : M a.`1 res].
+   have : Pr[C2.rest(p, a) @ &m : M (a.`1, res.`1) /\ M (a.`2, res.`2)] <=
+            Pr[C1.rest(p, a.`1) @ &m : M (a.`1, res)].
     rewrite H.
       have ->: a = (a.`1,a.`1).  smt. simplify.
       apply (avr_lemma_7_app &m M p ). 
@@ -191,41 +176,40 @@ qed.
 local lemma avr_lemma_9_app &m M p : 
      big (fun r => fst r = snd r)  (fun (c1c2 : ct * ct) => 
                   ((mu1 d c1c2.`1) * (mu1 d c1c2.`2)) * 
-                   Pr[ C1.rest(p,c1c2.`1) @ &m :  M c1c2.`1 res ]) 
-                   (cartprod2 allcs)
-     =   umc * Pr[ X1.run(p) @ &m :  M res.`1 res.`2 ].
-have ->: 
-       big (fun r => fst r = snd r)  (fun (c1c2 : ct * ct) => 
+                    Pr[ C1.rest(p,c1c2.`1) @ &m :  M (c1c2.`1, res) ]) 
+                    (cartprod2 allcs)
+     = (1%r/(size allcs)%r) * Pr[ X1.run(p) @ &m :  M (res.`1, res.`2) ].
+have ->: big (fun r => fst r = snd r)  (fun (c1c2 : ct * ct) => 
                   ((mu1 d c1c2.`1) * (mu1 d c1c2.`2)) * 
-                   Pr[ C1.rest(p,c1c2.`1) @ &m :  M c1c2.`1 res ]) 
+                   Pr[ C1.rest(p,c1c2.`1) @ &m :  M (c1c2.`1, res) ]) 
                    (cartprod2 allcs)
       = big (fun r => fst r = snd r)  (fun (c1c2 : ct * ct) => 
-                  umc * ((mu1 d c1c2.`1) * 
-                   Pr[ C1.rest(p,c1c2.`1) @ &m :  M c1c2.`1 res ])) 
+                  (1%r/(size allcs)%r) * ((mu1 d c1c2.`1) * 
+                   Pr[ C1.rest(p,c1c2.`1) @ &m :  M (c1c2.`1, res) ])) 
                    (cartprod2 allcs).
-apply eq_big. auto.
+apply eq_big. auto. 
 progress.
-rewrite ss. rewrite ss. auto. smt.
+rewrite ss. rewrite ss. simplify. auto. simplify. 
 have ->: big (fun (r : ct * ct) => r.`1 = r.`2)
   (fun (c1c2 : ct * ct) =>
-     umc * (mu1 d c1c2.`1 * Pr[C1.rest(p, c1c2.`1) @ &m : M c1c2.`1 res]))
+     (1%r/(size allcs)%r) * (mu1 d c1c2.`1 * Pr[C1.rest(p, c1c2.`1) @ &m : M (c1c2.`1, res)]))
   (cartprod2 allcs)
- = umc * big (fun (r : ct * ct) => r.`1 = r.`2)
+ = (1%r/(size allcs)%r) * big (fun (r : ct * ct) => r.`1 = r.`2)
   (fun (c1c2 : ct * ct) =>
-      (mu1 d c1c2.`1 * Pr[C1.rest(p, c1c2.`1) @ &m : M c1c2.`1 res]))
+      (mu1 d c1c2.`1 * Pr[C1.rest(p, c1c2.`1) @ &m : M (c1c2.`1, res)]))
   (cartprod2 allcs).
 rewrite mulr_sumr. auto.
 auto.
 have ->: big (fun (r : ct * ct) => r.`1 = r.`2)
   (fun (c1c2 : ct * ct) =>
-     mu1 d c1c2.`1 * Pr[C1.rest(p, c1c2.`1) @ &m : M c1c2.`1 res])
+     mu1 d c1c2.`1 * Pr[C1.rest(p, c1c2.`1) @ &m : M (c1c2.`1, res)])
   (cartprod2 allcs)
    = big predT
       (fun (c : ct) =>
-         mu1 d c * Pr[C1.rest(p, c) @ &m : M c res])
+         mu1 d c * Pr[C1.rest(p, c) @ &m : M (c, res)])
           allcs.
-have ->: big predT (fun (c : ct) => mu1 d c * Pr[C1.rest(p, c) @ &m : M c res]) allcs = big predT (fun (c : ct) => mu1 d c * Pr[C1.rest(p, c) @ &m : M c res]) 
-    (map fst (filter (fun x => fst x = snd x) (cartprod2 allcs))). rewrite kiki. smt. auto.
+have ->: big predT (fun (c : ct) => mu1 d c * Pr[C1.rest(p, c) @ &m : M (c, res)]) allcs = big predT (fun (c : ct) => mu1 d c * Pr[C1.rest(p, c) @ &m : M (c, res)]) 
+    (map fst (filter (fun x => fst x = snd x) (cartprod2 allcs))). rewrite cart2_diag_unzip1. smt. auto.
 rewrite big_mapT. 
 rewrite - big_filter. rewrite  /(\o). auto.
  rewrite x0. auto.
@@ -233,23 +217,146 @@ qed.
 
 
 local lemma avr_lemma_10_app &m M p : 
-  Pr[ Xseq(C2).run(p) @ &m  : res.`1.`1 <> res.`1.`2 /\ M res.`1.`1 res.`2.`1 /\ M res.`1.`2 res.`2.`2 ] >= 
-  Pr[ Xseq(C2).run(p) @ &m  : M res.`1.`1 res.`2.`1 /\ M res.`1.`2 res.`2.`2  ] 
-   - umc * Pr[ X1.run(p) @ &m :  M res.`1 res.`2 ].
+  Pr[ Xseq(C2).run(p) @ &m  : res.`1.`1 <> res.`1.`2 /\ M (res.`1.`1, res.`2.`1) /\ M (res.`1.`2, res.`2.`2) ] >= 
+  Pr[ Xseq(C2).run(p) @ &m  : M (res.`1.`1, res.`2.`1) /\ M (res.`1.`2, res.`2.`2)  ] 
+   - (1%r/(size allcs)%r) * Pr[ X1.run(p) @ &m :  M (res.`1, res.`2) ].
 rewrite - avr_lemma_9_app.
 apply avr_lemma_8_app.
 qed.
 
 
 local lemma avr_lemma_11_app &m M p : 
-   Pr[ Xseq(C2).run(p) @ &m  : res.`1.`1 <> res.`1.`2 /\ M res.`1.`1 res.`2.`1 /\ M res.`1.`2 res.`2.`2  ] 
-       >= Pr[ X1.run(p) @ &m :  M res.`1 res.`2 ] ^2
-          - umc * Pr[ X1.run(p) @ &m :  M res.`1 res.`2 ].
-apply (ler_trans (Pr[ Xseq(C2).run(p) @ &m  : M res.`1.`1 res.`2.`1 /\ M res.`1.`2 res.`2.`2  ] 
-   - umc * Pr[ X1.run(p) @ &m :  M res.`1 res.`2 ])). 
-   have ff : Pr[X1.run(p) @ &m : M res.`1 res.`2] ^ 2
-     <= Pr[Xseq(C2).run(p) @ &m : M res.`1.`1 res.`2.`1 /\ M res.`1.`2 res.`2.`2].
-   apply x2.
+   Pr[ Xseq(C2).run(p) @ &m  : res.`1.`1 <> res.`1.`2 
+            /\ M (res.`1.`1, res.`2.`1) /\ M (res.`1.`2, res.`2.`2) ] 
+       >= Pr[ X1.run(p) @ &m :  M (res.`1, res.`2) ] ^2
+          - (1%r/(size allcs)%r) * Pr[ X1.run(p) @ &m :  M (res.`1, res.`2) ].
+apply (ler_trans (Pr[ Xseq(C2).run(p) @ &m  : M (res.`1.`1, res.`2.`1) 
+                                             /\ M (res.`1.`2, res.`2.`2)  ] 
+   - (1%r/(size allcs)%r) * Pr[ X1.run(p) @ &m :  M (res.`1, res.`2) ])). 
+have ff : Pr[X1.run(p) @ &m : M (res.`1, res.`2)] ^ 2
+     <= Pr[Xseq(C2).run(p) @ &m : M (res.`1.`1, res.`2.`1) 
+                                     /\ M (res.`1.`2, res.`2.`2)].
+apply x2.
 smt. 
 apply (avr_lemma_10_app &m M p).
 qed.
+
+
+lemma final_eq &m M p : 
+   Pr[ InitRun2(A).run(p) @ &m 
+          : res.`1.`1 <> res.`2.`1 /\ M res.`1 /\ M res.`2 ] 
+  >= Pr[ InitRun1(A).run(p) @ &m  :  M res ]^2
+          - (1%r/(size allcs)%r) * Pr[ InitRun1(A).run(p) @ &m  :  M res ].
+proof.
+ have <-: Pr[ Xseq(C2).run(p) @ &m  : res.`1.`1 <> res.`1.`2 
+            /\ M (res.`1.`1, res.`2.`1) /\ M (res.`1.`2, res.`2.`2) ] 
+    = Pr[ InitRun2(A).run(p) @ &m 
+          : res.`1.`1 <> res.`2.`1 /\ M res.`1 /\ M res.`2 ].
+byequiv. proc.  simplify.
+swap {2} 2 -1.
+swap {2} 4 -2.
+inline*. wp. 
+call (_:true).
+call (_:true).
+call (_:true). wp.  simplify.
+rnd. rnd.
+skip. progress. auto.  auto.
+ have <-: Pr[ X1.run(p) @ &m :  M (res.`1, res.`2) ] 
+    = Pr[ InitRun1(A).run(p) @ &m : M res ].
+byequiv. proc. inline*. swap {2} 2 -1. wp. 
+simplify.   call (_:true).  call (_:true). wp. rnd. 
+skip. progress. auto.  auto.
+apply avr_lemma_11_app.
+qed.
+
+
+lemma final_eq_step1 &m AccRun SuccExtr p negl : 
+   Pr[ InitRun2(A).run(p) @ &m 
+          : res.`1.`1 <> res.`2.`1 /\ AccRun res.`1 /\ AccRun res.`2
+   /\ !SuccExtr res.`1 res.`2 ] <= negl
+  => 
+   Pr[ InitRun2(A).run(p) @ &m : res.`1.`1 <> res.`2.`1 
+                                 /\ AccRun res.`1 /\ AccRun res.`2 /\ SuccExtr res.`1 res.`2 ] 
+    >= (Pr[ InitRun1(A).run(p) @ &m  :  AccRun res ]^2
+         - (1%r/(size allcs)%r) * Pr[ InitRun1(A).run(p) @ &m  :  AccRun res ])
+    - negl.
+progress.
+have : Pr[InitRun1(A).run(p) @ &m : AccRun res] ^ 2 -
+  Pr[InitRun1(A).run(p) @ &m : AccRun res] / (size allcs)%r <=
+   Pr[InitRun2(A).run(p) @ &m : res.`1.`1 <> res.`2.`1 /\
+       AccRun res.`1 /\ AccRun res.`2 /\ SuccExtr res.`1 res.`2] + negl.
+  apply (ler_trans    Pr[ InitRun2(A).run(p) @ &m 
+          : res.`1.`1 <> res.`2.`1 /\ AccRun res.`1 /\ AccRun res.`2 ] ).
+  apply final_eq.  
+rewrite Pr[mu_split SuccExtr res.`1 res.`2]. 
+have ->: Pr[InitRun2(A).run(p) @ &m :
+   (res.`1.`1 <> res.`2.`1 /\ AccRun res.`1 /\ AccRun res.`2) /\
+   SuccExtr res.`1 res.`2] = Pr[InitRun2(A).run(p) @ &m :
+   res.`1.`1 <> res.`2.`1 /\ AccRun res.`1 /\ AccRun res.`2 /\
+   SuccExtr res.`1 res.`2].
+rewrite Pr[mu_eq]. smt. auto.
+have ->: Pr[InitRun2(A).run(p) @ &m :
+   (res.`1.`1 <> res.`2.`1 /\ AccRun res.`1 /\ AccRun res.`2) /\
+   !SuccExtr res.`1 res.`2] = Pr[InitRun2(A).run(p) @ &m :
+   res.`1.`1 <> res.`2.`1 /\ AccRun res.`1 /\ AccRun res.`2 /\
+   !SuccExtr res.`1 res.`2].
+rewrite Pr[mu_eq]. smt. auto.
+smt.
+smt.
+qed.
+
+
+require import RealExp.
+
+
+lemma qqq1  (a b : real) : a <= b  => sqrt a <= sqrt b.
+smt. qed.
+
+
+lemma qqq2  (a b : real) : a ^ 2 <= b  => a <= sqrt b.
+smt. qed.
+
+
+lemma final_eq_step2 &m AccRun SuccExtr p negl : 
+   Pr[ InitRun2(A).run(p) @ &m 
+          : res.`1.`1 <> res.`2.`1 /\ AccRun res.`1 /\ AccRun res.`2
+   /\ !SuccExtr res.`1 res.`2 ] <= negl
+ => Pr[ InitRun2(A).run(p) @ &m 
+          :  SuccExtr res.`1 res.`2 ] = 0%r   
+ => Pr[ InitRun1(A).run(p) @ &m  :  AccRun res ]
+   <=  sqrt (negl + 1%r/(size allcs)%r).
+proof.  progress.
+have f2 :     Pr[InitRun2(A).run(p) @ &m :
+       res.`1.`1 <> res.`2.`1 /\
+  AccRun res.`1 /\ AccRun res.`2 /\ SuccExtr res.`1 res.`2] = 0%r.
+  have ff2: Pr[InitRun2(A).run(p) @ &m :
+       res.`1.`1 <> res.`2.`1 /\
+  AccRun res.`1 /\ AccRun res.`2 /\ SuccExtr res.`1 res.`2]
+   <= 0%r. rewrite - H0.
+   rewrite Pr[mu_sub]. smt. auto. 
+  smt.
+have f1 :    0%r 
+    >= (Pr[ InitRun1(A).run(p) @ &m  :  AccRun res ]^2
+         - (1%r/(size allcs)%r) * Pr[ InitRun1(A).run(p) @ &m  :  AccRun res ])
+    - negl.
+rewrite - f2.
+apply (final_eq_step1 &m). assumption.
+clear f2. clear H.
+have f3 : Pr[InitRun1(A).run(p) @ &m : AccRun res] ^ 2 
+     <= 1%r / (size allcs)%r * Pr[InitRun1(A).run(p) @ &m : AccRun res] + negl.
+smt.
+clear f1.
+clear H0.
+have : Pr[InitRun1(A).run(p) @ &m : AccRun res] <=
+    sqrt (1%r / (size allcs)%r * Pr[InitRun1(A).run(p) @ &m : AccRun res] + negl).
+apply qqq2. auto.
+clear f3. simplify.
+move => f4.
+apply (ler_trans (sqrt (Pr[InitRun1(A).run(p) @ &m : AccRun res] / (size allcs)%r + negl))).
+auto.
+apply qqq1. smt.
+qed.
+
+
+end section.
+
