ZK_General_better.ec
@@ -1,0 +1,351 @@
+require import AllCore.
+
+require import AllCore Distr FSet StdRing StdOrder StdBigop List.
+(*---*) import RField RealOrder Bigreal BRA.
+
+require import Aux.
+
+type prob, wit, chal, com, resp, sbits, event.
+
+
+require While_not_b_proc.
+clone import While_not_b_proc as IF with type iat <- (prob * wit),
+                                         type rt <- bool.
+
+require While_Props.
+clone import While_Props as MW with type irt   <- prob,
+                                    type rrt   <- event * sbits,
+                                    type sbits <- sbits.
+import MW.IFB.
+import MW.IFB.IM.
+
+
+
+module type Prover = {
+  proc commit(x : prob, w : wit) : com
+  proc response(ch : chal) : resp
+}.
+
+module type Verifier = {
+  proc challenge(Ny : prob, c : com) : chal
+  proc verify(c : com, r : resp)     : bool
+  proc summitup(c : com, r : resp)   : sbits
+}.
+
+
+module type Simulator = {
+  proc run(Ny : prob) : event * sbits
+}.
+
+module type Dist = {
+  proc run(r:event * sbits) : bool
+}.
+
+
+
+section.
+
+declare module Sim1 : Simulator{DW, W}.
+declare module P : Prover.
+declare module V : Verifier.
+declare module D : Dist {Sim1}.
+
+
+axiom Sim1_ll : islossless Sim1.run.
+axiom D_ll : islossless D.run.
+axiom Sim1_run_rew x : hoare[ Sim1.run : (glob Sim1) = x ==> (glob Sim1) = x ].
+
+op fevent : event.
+op E : event * sbits -> bool.
+axiom  Estart :  E (fevent, witness) = false.
+
+local module W0 = {
+  proc run(a : prob ) = {
+      var r, b;
+      r <- Sim1.run(a);
+      b <- D.run(r);
+      return (b, r);
+  }
+}.
+
+local module W1 = {
+  module M = W(Sim1)
+  proc run(a : (event * sbits -> bool) * prob * int * int * (event * sbits) ) = {
+      var r, b;
+      r <- M.whp(a);
+      b <- D.run(r);
+      return (b, r);
+  }
+}.
+
+
+
+local lemma zk_step1 &m E p eps zkp:
+   `|Pr[ W0.run(p) @ &m : E res.`2 /\ res.`1]
+      / Pr[W0.run(p) @ &m : E res.`2] 
+        - zkp| <= eps
+  => 0%r <= eps 
+  => 0%r < Pr[W0.run(p) @ &m : E res.`2]
+  => exists (eps' : real),  0%r <= eps' <= eps  
+  /\ `|Pr[ W0.run(p) @ &m : E res.`2 /\ res.`1] 
+         / Pr[W0.run(p) @ &m : E res.`2] 
+                - zkp| = eps'
+  /\ (Pr[ W0.run(p) @ &m : E res.`2 /\ res.`1] 
+      = Pr[W0.run(p) @ &m : E res.`2]  
+        * (zkp - eps')
+      \/
+      Pr[ W0.run(p) @ &m : E res.`2 /\ res.`1] 
+      = Pr[W0.run(p) @ &m : E res.`2]  
+        * (zkp + eps')).
+proof.
+progress.
+apply oip3;auto.
+qed.
+
+
+local lemma zk_step2 &m E p ea :
+  Pr[ W1.run(E,p,1,ea,(fevent,witness)) 
+           @ &m : E res.`2 /\ res.`1 ]  
+     = big predT
+        (fun i => Pr[W0.run(p) @ &m : !E res.`2] ^ i 
+         * Pr[ W0.run(p) @ &m : E res.`2 /\  res.`1] )
+        (range 0 ea). 
+admitted.
+
+
+local lemma zk_step3 &m p eps ea coeff zkp:
+   `|Pr[ W0.run(p) @ &m : E res.`2 /\ res.`1]
+      / Pr[W0.run(p) @ &m : E res.`2] 
+        - zkp| <= eps
+  => 0%r < Pr[W0.run(p) @ &m : E res.`2]  
+  => 0%r <= eps 
+  => coeff = big predT
+               (fun i => Pr[W0.run(p) @ &m : !E res.`2] ^ i 
+                          * Pr[ W0.run(p) @ &m : E res.`2])
+               (range 0 ea) 
+  => exists (eps' : real), 
+    0%r <= eps' <= eps   /\ 
+     `|Pr[ W1.run(E, p,1,ea,(fevent,witness)) 
+           @ &m : E res.`2 /\ res.`1 ]  
+         - coeff * zkp| = coeff * eps'.
+proof. move => H0 H1 H2 coeffeq.
+have :  exists (eps' : real),  0%r <= eps' <= eps  
+  /\ `|Pr[ W0.run(p) @ &m : E res.`2 /\ res.`1] 
+         / Pr[W0.run(p) @ &m : E res.`2] 
+                - zkp| = eps'
+  /\ (Pr[ W0.run(p) @ &m : E res.`2 /\ res.`1] 
+      = Pr[W0.run(p) @ &m : E res.`2]  
+        * (zkp - eps')
+      \/
+      Pr[ W0.run(p) @ &m : E res.`2 /\ res.`1] 
+      = Pr[W0.run(p) @ &m : E res.`2]  
+        * (zkp + eps')).
+apply (zk_step1 &m). assumption. assumption. assumption.
+elim. move => eps' [H3 [H41 H42 ]].
+exists eps'. 
+split. auto.
+apply oip4.
+rewrite coeffeq.
+have ->: Pr[W0.run(p) @ &m : ! E res.`2]
+  = 1%r - Pr[W0.run(p) @ &m :  E res.`2].
+  have ->: 1%r = Pr[W0.run(p) @ &m :  true].
+  byphoare. 
+proc. call D_ll. call Sim1_ll. auto. auto. auto.
+  have ->: Pr[W0.run(p) @ &m : true] = Pr[W0.run(p) @ &m : E res.`2]
+   + Pr[W0.run(p) @ &m : !E res.`2]. rewrite Pr[mu_split E res.`2]. 
+  simplify. smt. smt.
+  have : 0%r <=
+bigi predT
+  (fun (i : int) =>
+     (1%r - Pr[W0.run(p) @ &m : E res.`2]) ^ i *
+     Pr[W0.run(p) @ &m : E res.`2]) 0 ea.
+  apply (big_geq0  Pr[W0.run(p) @ &m : E res.`2] _ ea). smt.
+  smt. 
+case (Pr[ W0.run(p) @ &m : E res.`2 /\ res.`1] 
+      = Pr[W0.run(p) @ &m : E res.`2]  
+        * (zkp + eps')).
+progress. rewrite /(\o).
+rewrite zk_step2. 
+rewrite H. simplify.
+have : bigi predT
+  (fun (i : int) =>
+     Pr[W0.run(p) @ &m : ! E res.`2] ^ i *
+     (Pr[W0.run(p) @ &m : E res.`2] *
+      (zkp + eps'))) 0 ea =
+coeff * zkp + coeff * eps'.
+rewrite coeffeq.
+rewrite mulr_suml.
+rewrite mulr_suml.
+rewrite - big_split.
+simplify. smt.
+timeout 20. smt.
+move => H5.
+have : Pr[ W0.run(p) @ &m : E res.`2 /\ res.`1] 
+        = Pr[W0.run(p) @ &m : E res.`2]  
+          * (zkp - eps').
+smt.
+progress. rewrite /(\o).
+rewrite zk_step2. 
+rewrite H. simplify.
+have : bigi predT
+  (fun (i : int) =>
+     Pr[W0.run(p) @ &m : ! E res.`2] ^ i *
+     (Pr[W0.run(p) @ &m : E res.`2] *
+      (zkp - eps'))) 0 ea =
+coeff * zkp - coeff * eps'.
+rewrite coeffeq.
+rewrite mulr_suml.
+rewrite mulr_suml.
+rewrite - big_split_min.
+simplify. smt.
+timeout 20. smt.
+qed.
+
+
+local module Iter(Sim1 : Simulator)  = {
+  module WI = W1
+  proc run(Ny : prob, ea : int, E : event * sbits -> bool) = {
+    var r;
+    r <@ WI.run(E,Ny,1,ea,(fevent,witness));
+    return r;
+  }
+}.
+
+
+
+local lemma zk_non_final &m p  eps ea coeff zkp:
+   `|Pr[ W0.run(p) @ &m : E res.`2 /\  res.`1] / Pr[W0.run(p) @ &m : E res.`2] 
+        - zkp| <= eps
+
+  => 0%r < Pr[W0.run(p) @ &m : E res.`2] 
+  => 0%r <= eps                 (* not needed *)
+  => coeff = big predT
+               (fun i => Pr[W0.run(p) @ &m : !E res.`2] ^ i 
+                          * Pr[ W0.run(p) @ &m : E res.`2])
+               (range 0 ea) 
+  => `|Pr[ Iter(Sim1).run(p,ea,E) 
+           @ &m : E res.`2 /\ res.`1 ]  
+              - coeff * zkp| <= eps.
+move => H1 H2 H3 H4.
+have ->: 
+  Pr[Iter(Sim1).run(p, ea, E) @ &m :
+     E res.`2 /\ res.`1]
+  = Pr[ W1.run(E,p,1,ea,(fevent,witness)) 
+           @ &m : E res.`2 /\ res.`1 ] .  
+ byequiv (_: _==> ={res}). proc*.
+inline Iter(Sim1).run. sp. wp. 
+call (_: ={glob Sim1, glob D}). simplify. sim. 
+skip. smt. auto. auto.
+have : coeff <= 1%r. 
+rewrite H4.
+have ->: Pr[W0.run(p) @ &m : ! E res.`2]
+  = 1%r - Pr[W0.run(p) @ &m :  E res.`2].
+  have ->: 1%r = Pr[W0.run(p) @ &m :  true].
+  byphoare. proc.  call D_ll. call Sim1_ll.  auto. auto. auto.
+  have ->: Pr[W0.run(p) @ &m : true] = Pr[W0.run(p) @ &m : E res.`2]
+   + Pr[W0.run(p) @ &m : !E res.`2]. rewrite Pr[mu_split E res.`2]. 
+  simplify. smt. smt.
+  have : 
+bigi predT
+  (fun (i : int) =>
+     (1%r - Pr[W0.run(p) @ &m : E res.`2]) ^ i *
+     Pr[W0.run(p) @ &m : E res.`2]) 0 ea <= 1%r.
+  apply (big_leq1  Pr[W0.run(p) @ &m : E res.`2] _ ea). smt.
+  smt.
+move => H6.
+have : exists eps', 0%r <= eps' <= eps /\ `|Pr[W1.run(E, p, 1, ea,
+                 (fevent, witness)) @ &m :
+     E res.`2 /\ res.`1] -
+  coeff * zkp| 
+  = coeff * eps'.
+apply (zk_step3 &m  p  eps ea coeff).
+auto.  assumption. auto. auto. auto.
+elim.
+move => eps' [eps'p1 epsp2].
+apply (ler_trans (coeff * eps')).
+smt.
+smt.
+qed.
+
+
+local lemma zk_almost_final &m p eps ea coeff zkp:
+   `|Pr[ W0.run(p) @ &m : E res.`2 /\ res.`1] / Pr[W0.run(p) @ &m : E res.`2] 
+        - zkp| <= eps
+  => 0%r < Pr[W0.run(p) @ &m : E res.`2] 
+  => coeff = big predT
+               (fun i => Pr[W0.run(p) @ &m : !E res.`2] ^ i 
+                         * Pr[ W0.run(p) @ &m : E res.`2])
+               (range 0 ea) 
+  => `|Pr[ Iter(Sim1).run(p,ea,E) 
+           @ &m : E res.`2 /\ res.`1 ]  
+         - zkp| <= eps + (1%r - coeff).
+proof.
+move => H1 H2 H3.
+have ie1 : `|Pr[ Iter(Sim1).run(p,ea,E) 
+           @ &m : E res.`2 /\  res.`1 ]  
+         - coeff * zkp| <= eps.
+apply (zk_non_final &m p eps ea coeff zkp);auto. smt.
+apply ots. admit.  admit.
+auto.
+qed.
+
+
+local lemma zk_final &m p eps ea zkp:
+   `|Pr[ W0.run(p) @ &m : E res.`2 /\ res.`1] 
+        / Pr[W0.run(p) @ &m : E res.`2] 
+        - zkp| <= eps
+  => 0%r < Pr[W0.run(p) @ &m : E res.`2] 
+  => 0 <= ea
+  => `|Pr[ Iter(Sim1).run(p,ea,E) 
+           @ &m : E res.`2 /\ res.`1 ]  
+         - zkp| 
+           <= eps + Pr[W0.run(p) @ &m : !E res.`2] ^ ea.
+proof. progress.
+have ->: Pr[W0.run(p) @ &m : !E res.`2] ^ ea
+ = 1%r - (1%r - Pr[W0.run(p) @ &m : !E res.`2] ^ ea).
+smt.
+rewrite - big_formula_p. smt. auto. progress.
+have ->: (1%r - Pr[W0.run(p) @ &m : ! E res.`2])
+ = Pr[W0.run(p) @ &m : E res.`2]. 
+have ->: 1%r = Pr[W0.run(p) @ &m :  true].
+byphoare. 
+proc.  call D_ll. call Sim1_ll. auto. auto. auto.
+have ->: Pr[W0.run(p) @ &m : true] = Pr[W0.run(p) @ &m : ! E res.`2]
+ + Pr[W0.run(p) @ &m : E res.`2]. rewrite Pr[mu_split ! E res.`2]. 
+simplify. smt. smt.
+apply (zk_almost_final &m);auto.
+qed.
+
+
+local lemma zk_final_le &m p p0 eps ea zkp:
+   `|Pr[ W0.run(p) @ &m : E res.`2 /\ res.`1] 
+        / Pr[W0.run(p) @ &m : E res.`2] 
+        - zkp| <= eps
+  => 0%r < Pr[W0.run(p) @ &m : E res.`2] 
+  => 0 <= ea
+  => Pr[W0.run(p) @ &m : E res.`2] >= p0
+  => `|Pr[ Iter(Sim1).run(p,ea,E) 
+           @ &m : E res.`2 /\ res.`1 ] - zkp| 
+              <= eps + (1%r-p0) ^ ea.
+proof. progress.
+have fff : p0 <= 1%r. smt.
+have f1 : `|Pr[ Iter(Sim1).run(p,ea,E) 
+           @ &m : E res.`2 /\ res.`1 ]  
+         - zkp| 
+      <= eps + (1%r - Pr[W0.run(p) @ &m : E res.`2] )^ea.
+have ->: (1%r - Pr[W0.run(p) @ &m : E res.`2] ) = 
+  (Pr[W0.run(p) @ &m : !E res.`2] ). 
+have ->: 1%r = Pr[W0.run(p) @ &m :  true].
+byphoare. proc. call D_ll. call Sim1_ll. auto. auto. auto.
+have ->: Pr[W0.run(p) @ &m : true] = Pr[W0.run(p) @ &m : ! E res.`2]
+ + Pr[W0.run(p) @ &m : E res.`2]. rewrite Pr[mu_split ! E res.`2]. 
+simplify. smt. smt.
+apply (zk_final &m).
+have f2 : 
+ 1%r - Pr[W0.run(p) @ &m : E res.`2] <= (1%r - p0).
+smt.
+have f3 : (1%r - Pr[W0.run(p) @ &m : E res.`2]) ^ ea <= (1%r - p0) ^ ea.
+apply multn2;auto. smt. auto. auto. auto.  smt.
+qed.
+
+end section.
